expressions.v
@@ -71,10 +71,16 @@ treatment by (Norrish, PhD thesis) and (Ellison/Rosu, 2012), as whenever a
 sequence point occurs, we only unlock the locations that have been locked by
 evaluating the sub-expression corresponding to that particular sequence point,
 instead of unlocking all locations. *)
+Inductive assign :=
+  | Assign (**i ordinary assignment *)
+  | PreOp : binop → assign (**i assignment operators and prefix increment,
+     decrement, etc. *)
+  | PostOp : binop → assign (**i postfix increment, decrement, etc. *).
+
 Inductive expr :=
   | EVar : nat → expr
   | EVal : indexset → val → expr
-  | EAssign : expr → expr → expr
+  | EAssign : assign → expr → expr → expr
   | ECall : funname → list expr → expr
   | ELoad : expr → expr
   | EAlloc : expr
@@ -82,6 +88,7 @@ Inductive expr :=
   | EUnOp : unop → expr → expr
   | EBinOp : binop → expr → expr → expr
   | EIf : expr → expr → expr → expr
+  | EComma : expr → expr → expr
   | ECast : int_type → expr → expr.
 
 (** We use the scope [expr_scope] to declare notations for expressions. We
@@ -94,7 +101,7 @@ Bind Scope expr_scope with expr.
 
 Arguments EVar _.
 Arguments EVal _ _%val_scope.
-Arguments EAssign _%expr_scope _%expr_scope.
+Arguments EAssign _ _%expr_scope _%expr_scope.
 Arguments ECall _ _%expr_scope.
 Arguments ELoad _%expr_scope.
 Arguments EAlloc.
@@ -102,15 +109,16 @@ Arguments EFree _%expr_scope.
 Arguments EUnOp _ _%expr_scope.
 Arguments EBinOp _ _%expr_scope _%expr_scope.
 Arguments EIf _%expr_scope _%expr_scope _%expr_scope.
+Arguments EComma _%expr_scope _%expr_scope.
 Arguments ECast _ _%expr_scope.
 
 Notation "'var' x" := (EVar x) (at level 10) : expr_scope.
 Notation "'valc' @{ Ω } v" := (EVal Ω v)
   (at level 10, format "'valc' @{ Ω }  v") : expr_scope.
 Notation "'valc' v" := (EVal ∅ v) (at level 10) : expr_scope.
-Notation "'voidc' @{ Ω }" := (EVal Ω voidc)
-  (at level 10, format "'voidc' @{ Ω }") : expr_scope.
-Notation "'voidc'" := (EVal ∅ voidc) : expr_scope.
+Notation "'indetc' @{ Ω }" := (EVal Ω indetc)
+  (at level 10, format "'indetc' @{ Ω }") : expr_scope.
+Notation "'indetc'" := (EVal ∅ indetc) : expr_scope.
 Notation "'intc' @{ Ω } x" := (EVal Ω (intc x))
   (at level 10, format "'intc' @{ Ω }  x") : expr_scope.
 Notation "'intc' x" := (EVal ∅ (intc x%Z)) : expr_scope.
@@ -120,7 +128,13 @@ Notation "'ptrc' b" := (EVal ∅ (ptrc b)) : expr_scope.
 Notation "'nullc' @{ Ω }" := (EVal Ω nullc)
   (at level 10, format "'nullc' @{ Ω }") : expr_scope.
 Notation "'nullc'" := (EVal ∅ nullc) : expr_scope.
-Infix "::=" := EAssign (at level 60) : expr_scope.
+Notation "el ::=@{ ass } er" := (EAssign ass el er)
+  (at level 60, format "el  ::=@{ ass }  er", right associativity) : expr_scope.
+Infix "::=" := (EAssign Assign) (at level 60, right associativity) : expr_scope.
+Infix "::⊙{ op }=" := (EAssign (PreOp op))
+  (at level 60, right associativity) : expr_scope.
+Infix "::=⊙{ op }" := (EAssign (PostOp op))
+  (at level 60, right associativity) : expr_scope.
 (* The infixes [++] and [::] are at level 60, [<$>] at 65. *)
 Notation "'call' f @ es" := (ECall f es)
   (at level 10, es at level 66) : expr_scope.
@@ -134,6 +148,8 @@ Notation "el ⊙{ op } er" := (EBinOp op el er)
 Notation "'IF' e 'then' el 'else' er" := (EIf e el er) : expr_scope.
 Notation "'cast' @{ τ } e" := (ECast τ e)
   (at level 10, format "'cast' @{ τ }  e") : expr_scope.
+Notation "el ,, er" := (EComma el er)
+  (at level 55, right associativity, format "el  ,,  er") : expr_scope.
 
 Infix "+" := (EBinOp PlusOp) : expr_scope.
 Infix "-" := (EBinOp MinusOp) : expr_scope.
@@ -151,6 +167,8 @@ Proof. by injection 1. Qed.
 Instance: Injective (=) (=) EFree.
 Proof. by injection 1. Qed.
 
+Instance assign_eq_dec: ∀ a1 a2 : assign, Decision (a1 = a2).
+Proof. solve_decision. Defined.
 Instance expr_eq_dec: ∀ e1 e2 : expr, Decision (e1 = e2).
 Proof.
   refine (fix go e1 e2 : Decision (e1 = e2) :=
@@ -158,8 +176,9 @@ Proof.
   | var i1, var i2 => cast_if (decide_rel (=) i1 i2)
   | valc@{Ω1} v1, valc@{Ω2} v2 =>
      cast_if_and (decide_rel (=) Ω1 Ω2) (decide_rel (=) v1 v2)
-  | el1 ::= er1, el2 ::= er2 => cast_if_and (decide_rel (=) el1 el2)
-     (decide_rel (=) er1 er2)
+  | el1 ::=@{ass1} er1, el2 ::=@{ass2} er2 =>
+     cast_if_and3 (decide_rel (=) ass1 ass2) (decide_rel (=) el1 el2)
+       (decide_rel (=) er1 er2)
   | call f1 @ es1, call f2 @ es2 => cast_if_and (decide_rel (=) f1 f2)
      (decide_rel (=) es1 es2)
   | load e1, load e2 => cast_if (decide_rel (=) e1 e2)
@@ -172,6 +191,8 @@ Proof.
   | (IF e1 then el1 else er1), (IF e2 then el2 else er2) =>
      cast_if_and3 (decide_rel (=) e1 e2)
        (decide_rel (=) el1 el2) (decide_rel (=) er1 er2)
+  | el1 ,, er1, el2 ,, er2 =>
+     cast_if_and (decide_rel (=) el1 el2) (decide_rel (=) er1 er2)
   | cast@{τ1} e1, cast@{τ2} e2 =>
      cast_if_and (decide_rel (=) τ1 τ2) (decide_rel (=) e1 e2)
   | _, _ => right _
@@ -180,13 +201,9 @@ Defined.
 
 (** The sequenced [||] and [&&] operators are defined in terms of the
 conditional. This keeps the expression language small. *)
-Definition EAnd (e1 e2 : expr) :=
-  (IF e1 then (IF e2 then intc int_true else intc int_false)
-  else intc int_false)%E.
+Definition EAnd (e1 e2 : expr) := (IF e1 then e2 else intc int_false)%E.
 Infix "&&" := EAnd : expr_scope.
-Definition EOr (e1 e2 : expr) :=
-  (IF e1 then intc int_true
-  else (IF e2 then intc int_true else intc int_false))%E.
+Definition EOr (e1 e2 : expr) := (IF e1 then intc int_true else e2)%E.
 Infix "||" := EOr : expr_scope.
 
 (** * Induction principles *)
@@ -198,7 +215,7 @@ Section expr_ind.
   Context (P : expr → Prop).
   Context (Pvar : ∀ x, P (var x)).
   Context (Pval : ∀ Ω v, P (valc@{Ω} v)).
-  Context (Passign : ∀ el er, P el → P er → P (el ::= er)).
+  Context (Passign : ∀ a el er, P el → P er → P (el ::=@{ a } er)).
   Context (Pcall : ∀ f es, Forall P es → P (call f @ es)).
   Context (Pload : ∀ e, P e → P (load e)).
   Context (Palloc : P alloc).
@@ -206,6 +223,7 @@ Section expr_ind.
   Context (Punop : ∀ op e, P e → P (⊙{op} e)).
   Context (Pbinop : ∀ op e1 e2, P e1 → P e2 → P (e1 ⊙{op} e2)).
   Context (Pif : ∀ e el er, P e → P el → P er → P (IF e then el else er)).
+  Context (Pcomma : ∀ el er, P el → P er → P (el ,, er)).
   Context (Pcast : ∀ τ e, P e → P (cast@{τ} e)).
 
   Definition expr_ind_alt : ∀ e, P e :=
@@ -213,7 +231,7 @@ Section expr_ind.
     match e with
     | var x => Pvar x
     | valc@{Ω} v => Pval Ω v
-    | el ::= er => Passign _ _ (go el) (go er)
+    | el ::=@{_} er => Passign _ _ _ (go el) (go er)
     | call f @ es => Pcall f es $ list_ind (Forall P)
        (Forall_nil_2 _) (λ e _, Forall_cons_2 _ _ _ (go e)) es
     | load e => Pload e (go e)
@@ -222,6 +240,7 @@ Section expr_ind.
     | ⊙{op} e => Punop op _ (go e)
     | el ⊙{op} er => Pbinop op _ _ (go el) (go er)
     | (IF e then el else er) => Pif _ _ _ (go e) (go el) (go er)
+    | el ,, er => Pcomma _ _ (go el) (go er)
     | cast@{τ} e => Pcast _ _ (go e)
     end%E.
 End expr_ind.
@@ -234,7 +253,7 @@ Instance expr_size: Size expr :=
   match e with
   | var _ => 0
   | valc@{_} _ => 0
-  | el ::= er => S (size el + size er)
+  | el ::=@{_} er => S (size el + size er)
   | call _ @ es => S (sum_list_with size es)
   | load e => S (size e)
   | alloc => 0
@@ -242,6 +261,7 @@ Instance expr_size: Size expr :=
   | ⊙{_} e => S (size e)
   | el ⊙{_} er => S (size el + size er)
   | (IF e then el else er) => S (size e + size el + size er)
+  | el ,, er => S (size el + size er)
   | cast@{_} e => size e
   end%E.
 
@@ -261,8 +281,8 @@ Qed.
 Inductive load_free: expr → Prop :=
   | EVar_load_free x : load_free (var x)
   | EVal_load_free Ω v : load_free (valc@{Ω} v)
-  | EAssign_load_free el er :
-     load_free el → load_free er → load_free (el ::= er)
+  | EAssign_load_free ass el er :
+     load_free el → load_free er → load_free (el ::=@{ass} er)
   | ECall_load_free f es : Forall load_free es → load_free (call f @ es)
   | EAlloc_load_free : load_free alloc
   | EFree_load_free e : load_free e → load_free (free e)
@@ -272,14 +292,16 @@ Inductive load_free: expr → Prop :=
   | EIf_load_free e el er :
      load_free e → load_free el → load_free er →
      load_free (IF e then el else er)
+  | EComma_load_free el er :
+     load_free el → load_free er →  load_free (el ,, er)
   | ECast_load_free τ e : load_free e → load_free (cast@{τ} e).
 
 Section load_free_ind.
   Context (P : expr → Prop).
   Context (Pvar : ∀ x, P (var x)).
   Context (Pval : ∀ Ω v, P (valc@{Ω} v)).
-  Context (Passign : ∀ el er,
-    load_free el → P el → load_free er → P er → P (el ::= er)).
+  Context (Passign : ∀ ass el er,
+    load_free el → P el → load_free er → P er → P (el ::=@{ass} er)).
   Context (Pcall : ∀ f es, Forall load_free es → Forall P es → P (call f @ es)).
   Context (Palloc : P alloc).
   Context (Pfree : ∀ e, load_free e → P e → P (free e)).
@@ -289,6 +311,8 @@ Section load_free_ind.
   Context (Pif : ∀ e el er,
     load_free e → P e → load_free el → P el → load_free er → P er →
     P (IF e then el else er)).
+  Context (Pcomma : ∀ el er,
+    load_free el → P el → load_free er → P er → P (el ,, er)).
   Context (Pcast : ∀ τ e, load_free e → P e → P (cast@{τ} e)).
 
   Definition load_free_ind_alt: ∀ e, load_free e → P e :=
@@ -296,7 +320,7 @@ Section load_free_ind.
     match H in load_free e return P e with
     | EVar_load_free x => Pvar _
     | EVal_load_free Ω v => Pval _ _
-    | EAssign_load_free _ _ Hl Hr => Passign _ _ Hl (go _ Hl) Hr (go _ Hr)
+    | EAssign_load_free _ _ _ Hl Hr => Passign _ _ _ Hl (go _ Hl) Hr (go _ Hr)
     | ECall_load_free _ _ H => Pcall _ _ H (Forall_impl _ _ _ H go)
     | EAlloc_load_free => Palloc
     | EFree_load_free _ H => Pfree _ H (go _ H)
@@ -305,6 +329,8 @@ Section load_free_ind.
        Pbinop _ _ _ H1 (go _ H1) H2 (go _ H2)
     | EIf_load_free _ _ _ H Hl Hr =>
        Pif _ _ _ H (go _ H) Hl (go _ Hl) Hr (go _ Hr)
+    | EComma_load_free _ _ Hl Hr =>
+       Pcomma _ _ Hl (go _ Hl) Hr (go _ Hr)
     | ECast_load_free _ _ H => Pcast _ _ H (go _ H)
     end.
 End load_free_ind.
@@ -316,15 +342,15 @@ Proof.
   match e return Decision (load_free e) with
   | var x => left _
   | valc@{_} _ => left _
-  | el ::= er => cast_if_and (go el) (go er)
+  | el ::=@{_} er => cast_if_and (go el) (go er)
   | call f @ es => cast_if (decide (Forall load_free es))
   | load e => right _
   | alloc => left _
   | free e => cast_if (go e)
   | ⊙{op} e => cast_if (go e)
   | el ⊙{op} er => cast_if_and (go el) (go er)
-  | (IF e then el else er) =>
-      cast_if_and3 (go e) (go el) (go er)
+  | (IF e then el else er) => cast_if_and3 (go e) (go el) (go er)
+  | EComma el er => cast_if_and  (go el) (go er)
   | cast@{_} e => cast_if (go e)
   end%E); first [by constructor | by inversion 1].
 Defined.
@@ -335,7 +361,7 @@ Instance expr_vars: Vars expr :=
   match e with
   | var n => {[ n ]}
   | valc@{_} _ => ∅
-  | el ::= er => vars el ∪ vars er
+  | el ::=@{_} er => vars el ∪ vars er
   | call _ @ es => ⋃ (vars <$> es)
   | alloc => ∅
   | load e
@@ -343,6 +369,7 @@ Instance expr_vars: Vars expr :=
   | ⊙{_} e => vars e
   | el ⊙{_} er => vars el ∪ vars er
   | (IF e then el else er) => vars e ∪ vars el ∪ vars er
+  | el ,, er => vars el ∪ vars er
   | cast@{_} e => vars e
   end%E.
 
@@ -352,7 +379,7 @@ Instance expr_funs: Funs expr :=
   match e with
   | var n => ∅
   | valc@{_} _ => ∅
-  | el ::= er => funs el ∪ funs er
+  | el ::=@{_} er => funs el ∪ funs er
   | call f @ es => {[ f ]} ∪ ⋃ (funs <$> es)
   | alloc => ∅
   | load e
@@ -360,6 +387,7 @@ Instance expr_funs: Funs expr :=
   | ⊙{_} e => funs e
   | el ⊙{_} er => funs el ∪ funs er
   | (IF e then el else er) => funs e ∪ funs el ∪ funs er
+  | el ,, er => funs el ∪ funs er
   | cast@{_} e => funs e
   end%E.
 
@@ -378,7 +406,7 @@ Instance expr_locks: Locks expr :=
   match e with
   | var n => ∅
   | valc@{Ω} _ => Ω
-  | el ::= er => locks el ∪ locks er
+  | el ::=@{_} er => locks el ∪ locks er
   | call _ @ es => ⋃ (locks <$> es)
   | alloc => ∅
   | load e
@@ -386,6 +414,7 @@ Instance expr_locks: Locks expr :=
   | ⊙{_} e => locks e
   | el ⊙{_} er => locks el ∪ locks er
   | (IF e then el else er) => locks e ∪ locks el ∪ locks er
+  | el ,, er => locks el ∪ locks er
   | cast@{_} e => locks e
   end%E.
 
@@ -408,6 +437,8 @@ Inductive is_pure (fs : funset) : expr → Prop :=
   | EIf_pure e el er :
      is_pure fs e → is_pure fs el → is_pure fs er →
      is_pure fs (IF e then el else er)
+  | EComma_pure el er :
+     is_pure fs el → is_pure fs er → is_pure fs (el ,, er)
   | ECast_pure τ e : is_pure fs e → is_pure fs (cast@{τ} e).
 
 Section is_pure_ind.
@@ -423,6 +454,8 @@ Section is_pure_ind.
   Context (Pif : ∀ e el er,
     is_pure fs e → P e → is_pure fs el → P el → is_pure fs er → P er →
     P (IF e then el else er)).
+  Context (Pcomma : ∀ el er,
+    is_pure fs el → P el → is_pure fs er → P er → P (el ,, er)).
   Context (Pcast : ∀ τ e, is_pure fs e → P e → P (cast@{τ} e)).
 
   Definition is_pure_ind_alt: ∀ e, is_pure fs e → P e :=
@@ -435,6 +468,7 @@ Section is_pure_ind.
     | EUnOp_pure _ _ H => Punop _ _ H (go _ H)
     | EBinOp_pure _ _ _ H1 H2 => Pbinop _ _ _ H1 (go _ H1) H2 (go _ H2)
     | EIf_pure _ _ _ H Hl Hr => Pif _ _ _ H (go _ H) Hl (go _ Hl) Hr (go _ Hr)
+    | EComma_pure _ _ Hl Hr => Pcomma _ _ Hl (go _ Hl) Hr (go _ Hr)
     | ECast_pure _ _ H => Pcast _ _ H (go _ H)
     end.
 End is_pure_ind.
@@ -452,6 +486,7 @@ Proof.
   | ⊙{op} e => cast_if (go e)
   | el ⊙{op} er => cast_if_and (go el) (go er)
   | (IF e then el else er) => cast_if_and3 (go e) (go el) (go er)
+  | el ,, er => cast_if_and (go el) (go er)
   | cast@{_} e => cast_if (go e)
   | _ => right _
   end%E); first [by subst; constructor | by inversion 1; subst].
@@ -472,7 +507,7 @@ Fixpoint expr_lift (e : expr) : expr :=
   match e with
   | var x => var (S x)
   | valc@{Ω} v => valc@{Ω} v
-  | el ::= er => el↑ ::= er↑
+  | el ::=@{ass} er => el↑ ::=@{ass} er↑
   | call f @ es => call f @ expr_lift <$> es
   | load e => load (e↑)
   | alloc => alloc
@@ -480,6 +515,7 @@ Fixpoint expr_lift (e : expr) : expr :=
   | ⊙{op} e => ⊙{op} e↑
   | el ⊙{op} er => el↑ ⊙{op} er↑
   | (IF e then el else er) => IF e↑ then el↑ else er↑
+  | el ,, er => el↑ ,, er↑
   | cast@{τ} e => cast@{τ} (e↑)
   end%E
 where "e ↑" := (expr_lift e) : expr_scope.
@@ -491,7 +527,8 @@ Inductive is_value : expr → Prop :=
   | EVal_is_value Ω v : is_value (valc@{Ω} v).
 Inductive is_redex : expr → Prop :=
   | EVar_is_redex x : is_redex (var x)
-  | EAssign_is_redex el er : is_value el → is_value er → is_redex (el ::= er)
+  | EAssign_is_redex ass el er :
+     is_value el → is_value er → is_redex (el ::=@{ass} er)
   | ECall_is_redex f es : Forall is_value es → is_redex (call f @ es)
   | ELoad_is_redex e : is_value e → is_redex (load e)
   | EAlloc_is_redex : is_redex alloc
@@ -500,6 +537,7 @@ Inductive is_redex : expr → Prop :=
   | EBinOp_is_redex op el er :
      is_value el → is_value er → is_redex (el ⊙{op} er)
   | EIf_is_redex e el er : is_value e → is_redex (IF e then el else er)
+  | EComma_is_redex el er : is_value el → is_redex (el ,, er)
   | ECast_is_redex τ e : is_value e → is_redex (cast@{τ} e).
 
 Instance is_value_dec (e : expr) : Decision (is_value e).
@@ -513,7 +551,7 @@ Proof.
   match e with
   | var _ => left _
   | valc@{_} _ => right _
-  | el ::= er => cast_if_and (decide (is_value el)) (decide (is_value er))
+  | el ::=@{_} er => cast_if_and (decide (is_value el)) (decide (is_value er))
   | call _ @ es => cast_if (decide (Forall is_value es))
   | alloc => left _
   | load e
@@ -521,6 +559,7 @@ Proof.
   | ⊙{_} e => cast_if (decide (is_value e))
   | el ⊙{_} er => cast_if_and (decide (is_value el)) (decide (is_value er))
   | (IF e then _ else _) => cast_if (decide (is_value e))
+  | el ,, er => cast_if (decide (is_value el))
   | cast@{_} e => cast_if (decide (is_value e))
   end%E); try (by constructor); abstract (by inversion 1).
 Defined.
@@ -548,8 +587,8 @@ Qed.
 contexts allow us to enforce an evaluation strategy. In particular, for the
 conditional we merely allow a hole for the first branch. *)
 Inductive ectx_item :=
-  | CAssignL : expr → ectx_item
-  | CAssignR : expr → ectx_item
+  | CAssignL : assign → expr → ectx_item
+  | CAssignR : assign → expr → ectx_item
   | CCall : funname → list expr → list expr → ectx_item
   | CLoad : ectx_item
   | CFree : ectx_item
@@ -557,13 +596,14 @@ Inductive ectx_item :=
   | CBinOpL : binop → expr → ectx_item
   | CBinOpR : binop → expr → ectx_item
   | CIf : expr → expr → ectx_item
+  | CComma : expr → ectx_item
   | CCast : int_type → ectx_item.
 Notation ectx := (list ectx_item).
 
 Bind Scope expr_scope with ectx_item.
 
-Arguments CAssignL _.
-Arguments CAssignR _.
+Arguments CAssignL _ _.
+Arguments CAssignR _ _.
 Arguments CCall _ _ _.
 Arguments CLoad.
 Arguments CFree.
@@ -571,11 +611,13 @@ Arguments CUnOp _.
 Arguments CBinOpL _ _.
 Arguments CBinOpR _ _.
 Arguments CIf _ _.
+Arguments CComma _.
 Arguments CCast _.
 
-Notation "□ ::= er" := (CAssignL er) (at level 60) : expr_scope.
-Notation "el ::= □" := (CAssignR el)
-  (at level 60, format "el  ::=  □") : expr_scope.
+Notation "□ ::=@{ a } er" := (CAssignL a er)
+  (at level 60, format "□  ::=@{ a }  er") : expr_scope.
+Notation "el ::=@{ a } □" := (CAssignR a el)
+  (at level 60, format "el  ::=@{ a }  □") : expr_scope.
 Notation "'call' f @ es1 □ es2" := (CCall f es1 es2)
   (at level 10, es1 at level 66, es2 at level 66) : expr_scope.
 Notation "'load' □" := CLoad (at level 10, format "load  □") : expr_scope.
@@ -588,6 +630,7 @@ Notation "el ⊙{ op } □" := (CBinOpR op el)
   (at level 50, format "el  ⊙{ op }  □") : expr_scope.
 Notation "'IF' □ 'then' el 'else' er" := (CIf el er)
   (at level 200, format "'IF'  □  'then'  el  'else'  er") : expr_scope.
+Notation "□ ,, er" := (CComma er) (at level 55, format "□  ,,  er") : expr_scope.
 Notation "'cast' @{ τ } □" := (CCast τ)
   (at level 10, format "'cast' @{ τ }  □") : expr_scope.
 
@@ -598,14 +641,15 @@ Proof. solve_decision. Defined.
 instances in the file [contexts], it is lifted to full expression contexts. *)
 Instance ectx_item_subst: Subst ectx_item expr expr := λ Ei e,
   match Ei with
-  | □ ::= er => e ::= er
-  | el ::= □ => el ::= e
+  | □ ::=@{ass} er => e ::=@{ass} er
+  | el ::=@{ass} □ => el ::=@{ass} e
   | call f @ es1 □ es2 => call f @ (reverse es1 ++ e :: es2)
   | load □ => load e
   | free □ => free e
   | ⊙{op} □ => ⊙{op} e
   | □ ⊙{op} er => e ⊙{op} er
   | el ⊙{op} □ => el ⊙{op} e
+  | □ ,, er => e ,, er
   | (IF □ then el else er) => IF e then el else er
   | cast @{τ} □ => cast @{τ} e
   end%E.
@@ -638,8 +682,8 @@ Qed.
 
 Instance ectx_locks: Locks ectx_item := λ Ei,
   match Ei with
-  | □ ::= er => locks er
-  | el ::= □ => locks el
+  | □ ::=@{_} er => locks er
+  | el ::=@{_} □ => locks el
   | call f @ es1 □ es2 => ⋃ (locks <$> es1) ∪ ⋃ (locks <$> es2)
   | load □ => ∅
   | free □ => ∅
@@ -647,6 +691,7 @@ Instance ectx_locks: Locks ectx_item := λ Ei,
   | □ ⊙{op} er => locks er
   | el ⊙{op} □ => locks el
   | (IF □ then el else er) => locks el ∪ locks er
+  | □ ,, er => locks er
   | cast @{τ} □ => ∅
   end%E.
 
@@ -683,8 +728,9 @@ Section ectx_expr_ind.
   Context (P : ectx → expr → Prop).
   Context (Pvar : ∀ E x, P E (var x)).
   Context (Pval : ∀ E Ω v, P E (valc@{Ω} v)).
-  Context (Passign : ∀ E el er,
-    P ((□ ::= er)%E :: E) el → P ((el ::= □)%E :: E) er → P E (el ::= er)).
+  Context (Passign : ∀ E ass el er,
+    P ((□ ::=@{ass} er)%E :: E) el → P ((el ::=@{ass} □)%E :: E) er →
+    P E (el ::=@{ass} er)).
   Context (Pcall : ∀ E f es,
     zipped_Forall (λ esl esr, P ((call f @ esl □ esr)%E :: E)) [] es →
     P E (call f @ es)).
@@ -697,6 +743,7 @@ Section ectx_expr_ind.
     P E (el ⊙{op} er)).
   Context (Pif : ∀ E e el er,
     P ((IF □ then el else er)%E :: E) e → P E (IF e then el else er)).
+  Context (Pcomma : ∀ E el er, P ((□ ,, er)%E :: E) el → P E (el ,, er)).
   Context (Pcast : ∀ E τ e,
     P ((cast @{τ} □)%E :: E) e → P E (cast @{τ} e)).
 
@@ -705,7 +752,7 @@ Section ectx_expr_ind.
     match e with
     | var x => Pvar _ x
     | valc@{Ω} v => Pval _ Ω v
-    | el ::= er => Passign _ _ _ (go _ el) (go _ er)
+    | el ::=@{_} er => Passign _ _ _ _ (go _ el) (go _ er)
     | call f @ es => Pcall E f es $
        zipped_list_ind _ zipped_Forall_nil
         (λ _ _ e, @zipped_Forall_cons _ (λ _ _, P _) _ _ _ (go _ e)) [] es
@@ -715,6 +762,7 @@ Section ectx_expr_ind.
     | ⊙{op} e => Punop _ op _ (go _ e)
     | el ⊙{op} er => Pbinop _ op _ _ (go _ el) (go _ er)
     | (IF e then el else er) => Pif _ _ _ _ (go _ e)
+    | el ,, er => Pcomma _ _ _ (go _ el)
     | cast @{τ} e => Pcast _ _ _ (go _ e)
     end%E.
 End ectx_expr_ind.
@@ -734,7 +782,7 @@ generic way. *)
 Inductive ectx_full : nat → Type :=
   | DCVal : indexset → val → ectx_full 0
   | DCVar : nat → ectx_full 0
-  | DCAssign : ectx_full 2
+  | DCAssign : assign → ectx_full 2
   | DCCall {n} : funname → ectx_full n
   | DCLoad : ectx_full 1
   | DCAlloc : ectx_full 0
@@ -742,11 +790,12 @@ Inductive ectx_full : nat → Type :=
   | DCUnOp : unop → ectx_full 1
   | DCBinOp : binop → ectx_full 2
   | DCIf : expr → expr → ectx_full 1
+  | DCComma : expr → ectx_full 1
   | DCCast : int_type → ectx_full 1.
 
 Arguments DCVal _ _.
 Arguments DCVar _.
-Arguments DCAssign.
+Arguments DCAssign _.
 Arguments DCCall {_} _.
 Arguments DCLoad.
 Arguments DCAlloc.
@@ -754,13 +803,14 @@ Arguments DCFree.
 Arguments DCUnOp _.
 Arguments DCBinOp _.
 Arguments DCIf _ _.
+Arguments DCComma _.
 Arguments DCCast _.
 
 Instance ectx_full_subst: DepSubst ectx_full (vec expr) expr := λ _ E,
   match E with
   | DCVal Ω v => λ _, valc@{Ω} v
   | DCVar x => λ _, var x
-  | DCAssign => λ es, es !!! 0 ::= es !!! 1
+  | DCAssign ass => λ es, es !!! 0 ::=@{ass} es !!! 1
   | DCCall _ f => λ es, call f @ es
   | DCLoad => λ es, load (es !!! 0)
   | DCAlloc => λ es, alloc
@@ -768,12 +818,14 @@ Instance ectx_full_subst: DepSubst ectx_full (vec expr) expr := λ _ E,
   | DCUnOp op => λ es, ⊙{op} es !!! 0
   | DCBinOp op => λ es, es !!! 0 ⊙{op} es !!! 1
   | DCIf el er => λ es, IF es !!! 0 then el else er
+  | DCComma er => λ es, es !!! 0 ,, er
   | DCCast τ => λ es, cast @{τ} (es !!! 0)
   end%E.
 Instance ectx_full_locks {n} : Locks (ectx_full n) := λ E,
   match E with
   | DCVal Ω v => Ω
   | DCIf el er => locks el ∪ locks er
+  | DCComma er => locks er
   | _ => ∅
   end%E.
 
@@ -797,9 +849,9 @@ Definition ectx_full_to_item {n} (E : ectx_full n)
   match E in ectx_full n return fin n → vec expr n → ectx_item with
   | DCVal _ _ => fin_0_inv _
   | DCVar _ => fin_0_inv _
-  | DCAssign =>
-     fin_S_inv _ (λ es, □ ::= es !!! 1)%E $
-     fin_S_inv _ (λ es, es !!! 0 ::= □)%E $ fin_0_inv _
+  | DCAssign ass =>
+     fin_S_inv _ (λ es, □ ::=@{ass} es !!! 1)%E $
+     fin_S_inv _ (λ es, es !!! 0 ::=@{ass} □)%E $ fin_0_inv _
   | DCCall _ f => λ i es, (call f @ reverse (take i es) □ drop (FS i) es)%E
   | DCLoad => fin_S_inv _ (λ es, load □)%E $ fin_0_inv _
   | DCAlloc => fin_0_inv _
@@ -809,6 +861,7 @@ Definition ectx_full_to_item {n} (E : ectx_full n)
      fin_S_inv _ (λ es, □ ⊙{op} es !!! 1)%E $
      fin_S_inv _ (λ es, es !!! 0 ⊙{op} □)%E $ fin_0_inv _
   | DCIf el er => fin_S_inv _ (λ es, IF □ then el else er)%E $ fin_0_inv _
+  | DCComma er => fin_S_inv _ (λ es, □ ,, er)%E $ fin_0_inv _
   | DCCast τ => fin_S_inv _ (λ es, cast@{τ} □)%E $ fin_0_inv _
   end i es.
 
@@ -886,7 +939,7 @@ Section expr_split.
     match e with
     | valc@{_} _ => ∅
     | var x => ∅ (* impossible *)
-    | el ::= er => go (□ ::= er :: E) el ∪ go (el ::= □ :: E) er
+    | el ::=@{ass} er => go (□ ::=@{ass} er :: E) el ∪ go (el ::=@{ass} □ :: E) er
     | call f @ es =>
        ⋃ zipped_map (λ esl esr, go ((call f @ esl □ esr) :: E)) [] es
     | load e => go (load □ :: E) e
@@ -895,6 +948,7 @@ Section expr_split.
     | ⊙{op} e => go (⊙{op} □ :: E) e
     | e1 ⊙{op} e2 => go (□ ⊙{op} e2 :: E) e1 ∪ go (e1 ⊙{op} □ :: E) e2
     | (IF e then el else er) => go ((IF □ then el else er) :: E) e
+    | el ,, er => go ((□ ,, er) :: E) el
     | cast@{τ} e => go ((cast@{τ} □) :: E) e
     end%E.
   Definition expr_redexes : expr → C := expr_redexes_go [].
